proofs/itrees/it_inlineI.v
@@ -1,0 +1,426 @@
+(* ** Imports and settings *)
+From Coq Require Import ZArith.
+From mathcomp Require Import ssreflect ssrfun ssrbool.
+Require Import expr compiler_util allocation.
+
+Local Open Scope seq_scope.
+
+Module Import E.
+
+  Definition pass : string := "inlining".
+
+  Definition inline_error msg := {|
+    pel_msg := msg;
+    pel_fn := None;
+    pel_fi := None;
+    pel_ii := None;
+    pel_vi := None;
+    pel_pass := Some pass;
+    pel_internal := true
+  |}.
+
+End E.
+
+(* ** inlining
+ * -------------------------------------------------------------------- *)
+
+Section INLINE.
+
+Context
+  {wsw : WithSubWord}
+  {asm_op syscall_state : Type}
+  {asmop: asmOp asm_op}
+  (rename_fd : instr_info -> funname -> ufundef -> ufundef)
+  (dead_vars_fd : ufun_decl -> instr_info -> Sv.t)
+.
+
+Definition get_flag (x:lval) flag :=
+  match x with
+  | Lvar x => if is_inline_var x then AT_inline else flag
+  | _      => flag
+  end.
+
+Definition assgn_tuple iinfo (xs:lvals) flag (tys:seq stype) (es:pexprs) :=
+  let assgn xe := MkI iinfo (Cassgn xe.1 (get_flag xe.1 flag) xe.2.1 xe.2.2) in
+  map assgn (zip xs (zip tys es)).
+
+Definition inline_c (inline_i: instr -> Sv.t -> cexec (Sv.t * cmd)) c s :=
+  foldr (fun i r =>
+    Let r := r in
+    Let ri := inline_i i r.1 in
+    ok (ri.1, ri.2 ++ r.2)) (ok (s,[::])) c.
+
+Definition sparams (fd:ufundef) :=
+  vrvs_rec Sv.empty (map Lvar fd.(f_params)).
+
+Definition locals_p (fd:ufundef) :=
+  let s := read_es (map Plvar fd.(f_res)) in
+  let w := write_c_rec s fd.(f_body) in
+  let r := read_c_rec w fd.(f_body) in
+  vrvs_rec r (map Lvar fd.(f_params)).
+
+Definition locals fd :=
+  Sv.diff (locals_p fd) (sparams fd).
+
+Definition check_rename f (fd1 fd2:ufundef) (s:Sv.t) :=
+  Let _ := check_ufundef dead_vars_fd tt tt (f,fd1) (f,fd2) tt in
+  let s2 := locals_p fd2 in
+  if disjoint s s2 then ok tt
+  else Error (inline_error (pp_s "invalid refreshing in function")).
+
+Definition get_fun (p:ufun_decls) (f:funname) :=
+  match get_fundef p f with
+  | Some fd => ok fd
+  | None    => Error (inline_error (pp_box [::pp_s "Unknown function"; PPEfunname f]))
+  end.
+
+Fixpoint inline_i (px: ufun_decls) (i:instr) (X:Sv.t) : cexec (Sv.t * cmd) :=
+  let '(MkI iinfo ir) := i in
+  match ir with
+  | Cassgn _ _ _ _
+  | Copn _ _ _ _
+  | Csyscall _ _ _
+    => ok (Sv.union (read_i ir) X, [::i])
+  | Cif e c1 c2  =>
+    Let c1 := inline_c (inline_i px) c1 X in
+    Let c2 := inline_c (inline_i px) c2 X in
+    ok (read_e_rec (Sv.union c1.1 c2.1) e, [::MkI iinfo (Cif e c1.2 c2.2)])
+  | Cfor x (d,lo,hi) c =>
+    let X := Sv.union (read_i ir) X in
+    Let c := inline_c (inline_i px) c X in
+    ok (X, [::MkI iinfo (Cfor x (d, lo, hi) c.2)])
+  | Cwhile a c e info c' =>
+    let X := Sv.union (read_i ir) X in
+    Let c := inline_c (inline_i px) c X in
+    Let c' := inline_c (inline_i px) c' X in
+    ok (X, [::MkI iinfo (Cwhile a c.2 e info c'.2)])
+  | Ccall xs f es =>
+    let X := Sv.union (read_i ir) X in
+    if ii_is_inline iinfo then
+      Let fd := add_iinfo iinfo (get_fun px f) in
+      let fd' := rename_fd iinfo f fd in
+      Let _ := add_iinfo iinfo (check_rename f fd fd' (Sv.union (vrvs xs) X)) in
+      let ii := ii_with_location iinfo in
+      let rename_args :=
+        assgn_tuple ii (map Lvar fd'.(f_params)) AT_rename fd'.(f_tyin) es
+      in
+      let rename_res :=
+        assgn_tuple ii xs AT_rename fd'.(f_tyout) (map Plvar fd'.(f_res))
+      in
+      ok (X, rename_args ++ fd'.(f_body) ++ rename_res)
+    else ok (X, [::i])
+  end.
+
+Definition inline_fd (p:ufun_decls) (fd:ufundef) :=
+  match fd with
+  | MkFun ii tyin params c tyout res ef =>
+    let s := read_es (map Plvar res) in
+    Let c := inline_c (inline_i p) c s in
+    ok (MkFun ii tyin params c.2 tyout res ef)
+  end.
+
+Definition inline_fd_cons (ffd:funname * ufundef) (p:cexec ufun_decls) :=
+  Let p := p in
+  let f := ffd.1 in
+  Let fd := add_funname f (add_finfo ffd.2.(f_info) (inline_fd p ffd.2)) in
+  ok ((f,fd):: p).
+
+Definition inline_prog (p:ufun_decls) :=
+  foldr inline_fd_cons (ok [::]) p.
+
+Definition inline_prog_err (p:uprog) :=
+  if uniq [seq x.1 | x <- p_funcs p] then
+    Let fds := inline_prog (p_funcs p) in
+    ok {| p_extra := p_extra p; p_globs := p_globs p; p_funcs := fds |}
+  else Error (inline_error (pp_s "two function declarations with the same name")).
+
+End INLINE. 
+
+(*******************************************************)
+
+From ITree Require Import
+     Basics
+     ITree
+     ITreeFacts
+     Events.Exception
+     Interp.Recursion
+     MonadState.
+Import Basics.Monads.
+
+Require Import it_sems_coreP.
+
+Require Import inline_lemmaI2.
+
+Require Import expr psem_defs psem_core it_exec tfam_iso.
+
+Section IT_section.
+
+Context
+  {asm_op: Type}
+  {wsw: WithSubWord}
+  {dc: DirectCall}
+  {syscall_state : Type}
+  {ep : EstateParams syscall_state}
+  {spp : SemPexprParams}
+  {sip : SemInstrParams asm_op syscall_state}
+  {pT : progT}
+  {scP : semCallParams}.
+
+Context
+  (rename_fd : instr_info -> funname -> ufundef -> ufundef)
+  (dead_vars_fd : ufun_decl -> instr_info -> Sv.t).
+
+Notation recCall := (callE (funname * fstate) fstate).
+
+Section IT_section1.
+
+Context {E E0} {wE : with_Error E E0} (* {sem_F : sem_Fun E } *)
+  (p : prog) (ev : extra_val_t).
+
+Definition flat_i_sem (i: instr) (s: estate) :
+  itree (recCall +' E) estate :=
+  isem_i_body p ev i s.
+
+Definition flat_cmd_sem (c: cmd) (s: estate) :
+  itree (recCall +' E) estate :=
+  isem_cmd_rec p ev c s.
+
+Definition flat_fun_sem (fn: funname) (fs: fstate) :
+  itree (recCall +' E) fstate :=
+  isem_fun_body p ev fn fs.
+
+Definition flat_fundef_sem (fd: fundef) (fs: fstate) :
+  itree (recCall +' E) fstate :=
+  isem_fundef_body p ev fd fs.
+
+Notation sem_inline it :=
+  (interp (ext_handler (handle_recCall p ev)) it).
+
+Notation RA_tr it :=
+  (translate (@rassoc_tr recCall recCall E) it).
+
+Definition handle_2recCall :
+  (recCall +' recCall) ~> itree ((recCall +' recCall) +' E) :=
+  joint_handler (handle_recCall p ev) (handle_recCall p ev). 
+
+Definition inline_i_info (i: instr) (c: cmd) : Type :=
+  let asem_i := flat_i_sem i in 
+  let asem_c := flat_cmd_sem c in
+  sig (fun (kt: estate -> itree ((recCall +' recCall) +' E) estate) =>
+    (forall s, eutt eq (forget_tr (kt s)) (asem_i s)) /\ 
+    (forall s, eutt eq (sem_inline (RA_tr (kt s))) (asem_c s))).
+
+Definition inline_ir_info (ir: instr_r) (ii: instr_info) (c: cmd) : Type :=
+  let asem_i := flat_i_sem (MkI ii ir) in 
+  let asem_c := flat_cmd_sem c in
+  sig (fun (kt: estate -> itree ((recCall +' recCall) +' E) estate) =>
+    (forall s, eutt eq (forget_tr (kt s)) (asem_i s)) /\
+    (forall s, eutt eq (sem_inline (RA_tr (kt s))) (asem_c s))).
+
+Definition inline_cmd_info (c1 c2: cmd) : Type :=
+  let asem_c1 := flat_cmd_sem c1 in 
+  let asem_c2 := flat_cmd_sem c2 in
+  sig (fun (kt: estate -> itree ((recCall +' recCall) +' E) estate) =>
+    (forall s, eutt eq (forget_tr (kt s)) (asem_c1 s)) /\
+    (forall s, eutt eq (sem_inline (RA_tr (kt s))) (asem_c2 s))).
+
+Lemma inline_cmd_x (px: ufun_decls) (c1: cmd) :
+  forall (X: Sv.t),
+  option (Sv.t * sigT (fun c2: cmd => inline_cmd_info c1 c2)).
+Proof.
+  set (Pr := fun ir => forall (ii: instr_info) (sv: Sv.t),
+               option (Sv.t * sigT (fun c2: cmd => inline_ir_info ir ii c2))).
+  set (Pi := fun i => forall (sv: Sv.t),
+                 option (Sv.t * sigT (fun c2: cmd => inline_i_info i c2))).
+  set (Pc := fun c1 => forall (sv: Sv.t),
+               option (Sv.t * sigT (fun c2: cmd => inline_cmd_info c1 c2))).  
+  set (CR := cmd_rect (Pr := Pr) (Pi := Pi) (Pc := Pc)).       
+  eapply CR.
+  
+  { intros ir ii H sv0; subst Pr Pi; simpl in *. 
+    destruct (H ii sv0) as [[sv [c2 H0]] | ].       
+    2: { exact None. }
+    unfold inline_ir_info in H0.
+    econstructor 1; split.
+    exact sv.
+    exists c2.
+    unfold inline_i_info.
+    exact H0.
+  }
+  
+  { intros sv0.
+    set C := inline_c (inline_i rename_fd dead_vars_fd px) [::] sv0.
+    simpl in *.                  
+    destruct C as [[sv c2] | ] eqn: was_C.
+    2: { exact None. }
+    inv was_C.
+    subst Pc; simpl.
+    econstructor 1; split.
+    exact sv.
+    exists [::].
+    unfold inline_cmd_info.
+    exists (fun s => Ret s); split; simpl; intro s.
+    { unfold forget_tr.
+      rewrite translate_ret; reflexivity.
+    }
+    { rewrite translate_ret.
+      rewrite interp_ret; reflexivity.
+    }
+  }
+
+  { intros i c Hi Hc sv0.
+    destruct (Hi sv0) as [[sv_i [c2_i Hi1]] | ].
+    2: { exact None. }
+    destruct (Hc sv_i) as [[sv_c [c2_c Hc1]] | ]. 
+    2: { exact None. }
+    econstructor 1.
+    split.
+    exact sv_c.
+    exists (c2_i ++ c2_c).
+    unfold inline_i_info, inline_cmd_info in Hi1, Hc1.
+    unfold inline_cmd_info. 
+    destruct Hi1 as [kt1 [Hi1 Hi2]].
+    destruct Hc1 as [kt2 [Hc1 Hc2]].
+
+    set it3 := (fun s => bind (kt1 s) kt2).
+    exists it3; split; simpl; intro s; subst it3; unfold forget_tr.
+
+    { rewrite translate_bind.
+      eapply eqit_bind; eauto.
+      eapply Hi1.
+    }
+    { rewrite translate_bind.
+      setoid_rewrite isem_cmd_cat; simpl.
+      rewrite interp_bind.
+      eapply eqit_bind; eauto.
+      eapply Hi2.
+    }
+  }
+
+  { intros x tg ty e.
+    subst Pr; simpl; intros ii sv0.
+    econstructor 1; split.
+    exact sv0.
+    exists ( [:: (MkI ii (Cassgn x tg ty e))] ).
+    unfold inline_ir_info.
+    set kt := (fun s => @free_tr recCall recCall E _
+                          (flat_i_sem (MkI ii (Cassgn x tg ty e)) s)).
+    exists kt; split; subst kt; simpl; intro s.
+    { rewrite <- forget_free_inv_lemma.
+      reflexivity.
+    }
+    { setoid_rewrite <- rassoc_free_interp_lemma at 1.
+      setoid_rewrite bind_ret_r.
+      reflexivity.
+    }
+  }
+
+  { intros xs t o es.
+    subst Pr; simpl; intros ii sv0.
+    econstructor 1; split.
+    exact sv0.
+    exists ( [:: (MkI ii (Copn xs t o es))] ).
+    unfold inline_ir_info.
+    set kt := (fun s => @free_tr recCall recCall E _
+                          (flat_i_sem (MkI ii (Copn xs t o es)) s)).
+    exists kt; split; subst kt; simpl; intro s.
+    { rewrite <- forget_free_inv_lemma.
+      reflexivity.
+    }
+    { setoid_rewrite <- rassoc_free_interp_lemma at 1.
+      setoid_rewrite bind_ret_r.
+      reflexivity.
+    }
+  }
+
+  { intros xs o es.
+    subst Pr; simpl; intros ii sv0.
+    econstructor 1; split.
+    exact sv0.
+    exists ( [:: (MkI ii (Csyscall xs o es))] ).
+    unfold inline_ir_info.
+    set kt := (fun s => @free_tr recCall recCall E _
+                          (flat_i_sem (MkI ii (Csyscall xs o es)) s)).
+    exists kt; split; subst kt; simpl; intro s.
+    { rewrite <- forget_free_inv_lemma.
+      reflexivity.
+    }
+    { setoid_rewrite <- rassoc_free_interp_lemma at 1.
+      setoid_rewrite bind_ret_r.
+      reflexivity.
+    }
+  }
+
+  { rename c1 into c0.
+    intros e c1 c2 Hc1 Hc2.
+    subst Pr; simpl; intros ii sv0.
+    unfold Pc in Hc1, Hc2.
+    
+    destruct (Hc1 sv0) as [[sv1 [c1R [kt1 [Hc1A Hc1B]]]] | ].
+    2: { exact None. }
+    destruct (Hc2 sv0) as [[sv2 [c2R [kt2 [Hc2A Hc2B]]]] | ].
+    2: { exact None. }
+
+    set svR := (read_e_rec (Sv.union sv1 sv2) e).
+    econstructor 1; split.
+    exact svR.
+
+    exists ([::MkI ii (Cif e c1R c2R)]).
+    unfold inline_ir_info.
+
+    admit.
+  }
+
+  { rename c1 into c0.
+    intros x dir lo hi c Hc.
+    subst Pr; simpl; intros ii sv0.
+    unfold Pc in Hc.
+    
+    destruct (Hc sv0) as [[sv1 [c1R [kt1 [Hc1A Hc1B]]]] | ].
+    2: { exact None. }
+
+    set ir := (Cfor x (dir, lo, hi) c0).
+    
+    set svR := Sv.union (read_i ir) sv0.
+    econstructor 1; split.
+    exact svR.
+
+    exists ([::MkI ii (Cfor x (dir, lo, hi) c1R)]).
+    unfold inline_ir_info.
+
+    admit.
+  }
+
+  { rename c1 into c0.
+    intros a c1 e ii2 c2 Hc1 Hc2.
+    subst Pr; simpl; intros ii sv0.
+    unfold Pc in Hc1, Hc2.
+    
+    destruct (Hc1 sv0) as [[sv1 [c1R [kt1 [Hc1A Hc1B]]]] | ].
+    2: { exact None. }
+    destruct (Hc2 sv0) as [[sv2 [c2R [kt2 [Hc2A Hc2B]]]] | ].
+    2: { exact None. }
+
+    econstructor 1; split.
+    exact sv0.
+
+    exists ([::MkI ii (Cwhile a c1R e ii2 c2R)]).
+    unfold inline_ir_info.
+
+    admit.
+  }
+
+  { rename c1 into c0.
+    intros xs fn es.
+    subst Pr; simpl; intros ii sv0.
+
+    admit.
+  }
+
+Admitted.
+
+
+End IT_section1.
+    
+End IT_section.
+  
